Makefile
@@ -80,19 +80,21 @@ $(COQ_DIR)/RBTree.vo: $(COQ_DIR)/RBTree.v
 $(COQ_DIR)/TreeRep.vo: $(COQ_DIR)/TreeRep.v $(COQ_DIR)/RBTree.vo
 	$(COQC) $(COQFLAGS) $<
 
-$(COQ_DIR)/FindSpec.vo: $(COQ_DIR)/FindSpec.v $(COQ_DIR)/RBTree.vo $(COQ_DIR)/TreeRep.vo $(COQ_DIR)/map_int_int_cpp.vo
+$(COQ_DIR)/FindSpec.vo: $(COQ_DIR)/FindSpec.v $(COQ_DIR)/RBTree.vo $(COQ_DIR)/TreeRep.vo
 	$(COQC) $(COQFLAGS) $<
 
-$(COQ_DIR)/InsertSpec.vo: $(COQ_DIR)/InsertSpec.v $(COQ_DIR)/RBTree.vo $(COQ_DIR)/TreeRep.vo $(COQ_DIR)/map_int_int_cpp.vo
+$(COQ_DIR)/InsertSpec.vo: $(COQ_DIR)/InsertSpec.v $(COQ_DIR)/RBTree.vo $(COQ_DIR)/TreeRep.vo
 	$(COQC) $(COQFLAGS) $<
 
-$(COQ_DIR)/RefCount.vo: $(COQ_DIR)/RefCount.v $(COQ_DIR)/RBTree.vo $(COQ_DIR)/TreeRep.vo $(COQ_DIR)/map_int_int_cpp.vo
+$(COQ_DIR)/RefCount.vo: $(COQ_DIR)/RefCount.v $(COQ_DIR)/RBTree.vo $(COQ_DIR)/TreeRep.vo
 	$(COQC) $(COQFLAGS) $<
 
-$(COQ_DIR)/Invariants.vo: $(COQ_DIR)/Invariants.v $(COQ_DIR)/RBTree.vo $(COQ_DIR)/TreeRep.vo
+$(COQ_DIR)/Invariants.vo: $(COQ_DIR)/Invariants.v $(COQ_DIR)/RBTree.vo
 	$(COQC) $(COQFLAGS) $<
 
-proofs: $(COQ_DIR)/RBTree.vo $(COQ_DIR)/TreeRep.vo
+proofs: $(COQ_DIR)/RBTree.vo $(COQ_DIR)/TreeRep.vo \
+        $(COQ_DIR)/FindSpec.vo $(COQ_DIR)/InsertSpec.vo \
+        $(COQ_DIR)/RefCount.vo $(COQ_DIR)/Invariants.vo
 
 # ---- Cleanup ----
 
